examples/struct/keyvalue.pos/Test.fst
@@ -1,7 +1,0 @@
-module Test
-
-open KeyValue
-open PureParser
-open Validator
-open PureEncoder
-open Serializer
